# baseURI: https://w3id.org/exdoc
# prefix: exdoc

@prefix dc: <http://purl.org/dc/terms/> .
@prefix exdoc: <https://w3id.org/exdoc#> .
@prefix foaf: <http://xmlns.com/foaf/0.1/> .
@prefix owl: <http://www.w3.org/2002/07/owl#> .
@prefix rdf: <http://www.w3.org/1999/02/22-rdf-syntax-ns#> .
@prefix rdfs: <http://www.w3.org/2000/01/rdf-schema#> .
@prefix sdo: <https://schema.org/> .
@prefix skos: <http://www.w3.org/2004/02/skos/core#> .
@prefix vann: <http://purl.org/vocab/vann/> .
@prefix voaf: <http://purl.org/vocommons/voaf#> .
@prefix xsd: <http://www.w3.org/2001/XMLSchema#> .

<https://w3id.org/exdoc>
  rdf:type voaf:Vocabulary ;
  rdf:type owl:Ontology ;
  dc:creator [
      rdf:type sdo:Person ;
      sdo:email <mailto:philipp.hagedorn-n6v@rub.de> ;
      sdo:identifier <https://orcid.org/0000-0002-6249-243X> ;
      sdo:memberOf [
          sdo:identifier <https://www.inf.bi.ruhr-uni-bochum.de/iib/lehrstuhl/mitarbeiter/philipp_hagedorn.html.en> ;
          sdo:name "Ruhr University Bochum" ;
        ] ;
      sdo:name "Philipp Hagedorn" ;
    ] ;
  dc:description """This ontology provides an extension for document types for the [ISO 21597 ICDD Part 1](https://www.iso.org/standard/74389.html)  Container ontology `ct: <`[https://standards.iso.org/iso/21597/-1/ed-1/en/Container#](https://standards.iso.org/iso/21597/-1/ed-1/en/Container.rdf)`>`.

The preferred namespace prefix is `exdoc` for the namespace IRI [https://w3id.org/exdoc](https://w3id.org/exdoc).  

It includes the [ExternalDatabase](#ExternalDatabase) class as a subclass of the `ct:ExternalDocument`. This class can be used to provide information and connection details from an existing relational database, e.g., to retrieve data from DB and convert it into payload triples using R2RML mappings (see [W3C R2RML Recommendation](https://www.w3.org/TR/r2rml/)). When working with databases in ICDD container, be sure you do not store credentials for the database in the connection string but in a secure credentials store. 

It also includes the [PayloadProxy](#PayloadProxy) class as a subclass of the `ct:ExternalDocument` class for registering payload triples from the \"payload triples\" folder. Instances of these classes can be used to define link elements for RDF-based data in ICDD containers."""@en-GB ;
  dc:issued "2021-05-08"^^xsd:date ;
  dc:license <https://creativecommons.org/licenses/by/4.0/> ;
  dc:modified "2022-08-02"^^xsd:date ;
  dc:publisher [
      rdf:type foaf:Organization ;
      foaf:homepage <http://www.inf.bi.rub.de> ;
      foaf:name "Lehrstuhl Informatik im Bauwesen" ;
    ] ;
  dc:rights "Copyright 2022 by Chair of Computing in Engineering, Ruhr University Bochum" ;
  dc:source <https://github.com/RUB-Informatik-im-Bauwesen/exdoc> ;
  dc:title "Extension for document types for the ISO 21597 ICDD Part 1 Container ontology"@en-GB ;
  vann:preferredNamespacePrefix "exdc" ;
  vann:preferredNamespaceUri <https://w3id.org/exdoc> ;
  owl:versionIRI <https://w3id.org/exdoc> ;
  owl:versionInfo "v0.4" ;
  skos:historyNote """
  v0.3: adding `PayloadProxy` class

  v0.3: adding `databaseMapping` reference

  v0.2: adding `databaseType` and `databaseQueryLanguage`

  v0.1: initial ontology

  """ ;
.
exdoc:ExternalDatabase
  rdf:type owl:Class ;
  rdfs:comment "a proxy document referencing to an external data source with a connection string"@en-GB ;
  rdfs:label "External Database"@en-GB ;
  rdfs:subClassOf <https://standards.iso.org/iso/21597/-1/ed-1/en/Container#ExternalDocument> ;
  rdfs:subClassOf [
      rdf:type owl:Restriction ;
      owl:cardinality "1"^^xsd:nonNegativeInteger ;
      owl:onProperty exdoc:databaseConnectionString ;
    ] ;
  rdfs:subClassOf [
      rdf:type owl:Restriction ;
      owl:cardinality "1"^^xsd:nonNegativeInteger ;
      owl:onProperty exdoc:databaseName ;
    ] ;
  rdfs:subClassOf [
      rdf:type owl:Restriction ;
      owl:cardinality "1"^^xsd:nonNegativeInteger ;
      owl:onProperty exdoc:databaseQueryLanguage ;
    ] ;
  rdfs:subClassOf [
      rdf:type owl:Restriction ;
      owl:cardinality "1"^^xsd:nonNegativeInteger ;
      owl:onProperty exdoc:databaseType ;
    ] ;
  rdfs:subClassOf [
      rdf:type owl:Restriction ;
      owl:maxCardinality "1"^^xsd:nonNegativeInteger ;
      owl:onProperty exdoc:databaseMapping ;
    ] ;
  owl:disjointWith exdoc:PayloadProxy ;
.
exdoc:PayloadProxy
  rdf:type owl:Class ;
  rdfs:comment "a proxy document referencing to payload triples using the base uri of the triples file"@en-GB ;
  rdfs:label "Payload Proxy"@en-GB ;
  rdfs:subClassOf <https://standards.iso.org/iso/21597/-1/ed-1/en/Container#ExternalDocument> ;
  rdfs:subClassOf [
      rdf:type owl:Restriction ;
      owl:cardinality "1"^^xsd:nonNegativeInteger ;
      owl:onProperty <https://standards.iso.org/iso/21597/-1/ed-1/en/Container#url> ;
    ] ;
  owl:disjointWith exdoc:ExternalDatabase ;
.
exdoc:databaseConnectionString
  rdf:type owl:DatatypeProperty ;
  rdfs:comment "A database connection string is a string that specifies information about a data source and the means of connecting to it from an ICDD. It can be passed to an underlying driver or provider in order to initiate the connection. Warning: The connection string holds sensitive information."@en-GB ;
  rdfs:domain exdoc:ExternalDatabase ;
  rdfs:label "connection string"@en-GB ;
  rdfs:range xsd:string ;
.
exdoc:databaseMapping
  rdf:type owl:ObjectProperty ;
  rdfs:comment "The mapping file, which allows for the generation of structured RDF-based data from the specified database. This file also needs to be specified within the respective container."@en-GB ;
  rdfs:domain exdoc:ExternalDatabase ;
  rdfs:label "database mapping"@en-GB ;
  rdfs:range <https://standards.iso.org/iso/21597/-1/ed-1/en/Container#Document> ;
.
exdoc:databaseName
  rdf:type owl:DatatypeProperty ;
  rdfs:comment "The database name is used to adress the correct mapping from the mapping file to a certain database within the connection string."@en-GB ;
  rdfs:domain exdoc:ExternalDatabase ;
  rdfs:label "database name"@en-GB ;
  rdfs:range xsd:string ;
  rdfs:subPropertyOf <https://standards.iso.org/iso/21597/-1/ed-1/en/Container#name> ;
.
exdoc:databaseQueryLanguage
  rdf:type owl:DatatypeProperty ;
  rdfs:comment "The query language, which can be used to retrieve information from the specified database."@en-GB ;
  rdfs:label "query language"@en-GB ;
  rdfs:range xsd:string ;
.
exdoc:databaseType
  rdf:type owl:DatatypeProperty ;
  rdfs:comment "The type of database that is specified, e.g. MySQL, NoSQL, and others."@en-GB ;
  rdfs:domain exdoc:ExternalDatabase ;
  rdfs:label "database type"@en-GB ;
  rdfs:range xsd:string ;
.
